\section{Sampling and Reconstruction} 

\subsection{$x_s(t)$}

\begin{eqnarray*}
x_s(t) & = & x_c(t) \* s(t) \\
       & = & x_c(t) \* T \sum_{n=-\infty}^{\infty} \delta (t-nT) \\
       & \overset{\text{masking prop.}}{=}  & T \sum_{n=-\infty}^{\infty} x_c(nT) \* \delta (t-nT)
\end{eqnarray*}


\subsection{$X_s(j\Omega)$}

Fourier Series of $s(t)$:

\begin{eqnarray*}
s(t) & = & \sum_{k=-\infty}^{\infty} A_k \* e^{j2\pi k t \* \frac{1}{T}}
\end{eqnarray*}

\begin{eqnarray*}
A_k & = & \frac{1}{T} \int_{-\frac{T}{2}}^{\frac{T}{2}} T \sum_{n=-\infty}^{\infty} \underbrace{\delta (t-nT) e^{-j \frac{2\pi}{T}kt}}_{\text{masking property}}  dt \\
& = & \frac{T}{T} \int_{-\frac{T}{2}}^{\frac{T}{2}} \sum_{n=-\infty}^{\infty} \delta (t-nT) e^{-j \frac{2\pi}{T}k\* nT} dt \\
& = & \sum_{n=-\infty}^{\infty}  e^{-j \frac{2\pi}{T}k\* nT} \underbrace{\int_{-\frac{T}{2}}^{\frac{T}{2}}  \delta (t-nT) dt}_{\text{1 for n=0, 0 else}} \\
& = & e^{-j 2 \pi k 0 } = 1 \quad \forall k
\end{eqnarray*}

With $\Omega_s = \frac{2\pi}{T}$ $s(t)$ can be written as
\begin{eqnarray*}
s(t) & = & \sum_{k=-\infty}^{\infty} e^{j \Omega_s k t}
\end{eqnarray*}

Now the representation as Fourier Series can be transformed to the frequency domain.

\begin{eqnarray*}
S(j\Omega) & = & \int_{-\infty}^{\infty} s(t) \* e^{-j \Omega t} dt \\
 & = & \int_{-\infty}^{\infty} \sum_{k=-\infty}^{\infty} e^{j \Omega_s k t} \* e^{-j \Omega t} dt \\
 & = & \sum_{k=-\infty}^{\infty}  \int_{-\infty}^{\infty} e^{j \Omega_s k t} \* e^{-j \Omega t} dt 
\end{eqnarray*}

$e^{j \Omega_s k t}$ can be exchanged by
\begin{eqnarray*}
e^{j \Omega_s k t} =  \int_{-\infty}^{\infty} \delta(\Omega - k\Omega_s) e^{j \Omega t} dt
\end{eqnarray*}
due to the masking property of the delta impulse. This leads to

\begin{eqnarray*}
S(j\Omega) & = & \sum_{k=-\infty}^{\infty}  \int_{-\infty}^{\infty} \int_{-\infty}^{\infty} \delta(\Omega - k\Omega_s) e^{j \Omega t} dt \* e^{-j \Omega t} dt \\
S(j\Omega) & = & \sum_{k=-\infty}^{\infty}  \int_{-\infty}^{\infty} \int_{-\infty}^{\infty} \delta(\Omega - k\Omega_s) e^{j \Omega t} \* e^{-j \Omega t} dt dt \\
S(j\Omega) & = & \sum_{k=-\infty}^{\infty}  \int_{-\infty}^{\infty} \int_{-\infty}^{\infty} \delta(\Omega - k\Omega_s) \underbrace{e^{j (\Omega t-\Omega t)}}_{=1} dt dt \\
S(j\Omega) & = & \sum_{k=-\infty}^{\infty} \delta(\Omega - k\Omega_s)
\end{eqnarray*}

In order to get $X_s(j\Omega)$, $X_c(j\Omega)$ and $S(j\Omega)$ are convoluted
\begin{eqnarray*}
X_s(j\Omega) & = & X_c(j\Omega) \ast S(j\Omega) \\
X_s(j\Omega) & = & X_c(j\Omega) \ast \sum_{k=-\infty}^{\infty} \delta(\Omega - k\Omega_s) \\
X_s(j\Omega) & \overset{\text{shifting prop.}}{=} & \sum_{k=-\infty}^{\infty} X_c(j(\Omega-k\Omega_s) )
\end{eqnarray*}


